src/Dafny/examples/fs/byte_fs2.dfy
@@ -1,0 +1,170 @@
+include "block_fs.dfy"
+
+module ByteFs {
+  import Fs
+  import opened BlockFs
+  import IndirectPos
+  import opened IndFs
+  import opened FsKinds
+  import opened JrnlTypes
+  import opened JrnlSpec
+  import opened Machine
+  import opened ByteSlice
+  import Inode
+
+  function num_used(sz: nat): nat
+  {
+    sz / 4096
+  }
+
+  function {:opaque} raw_inode_data(d: InodeData): (bs:seq<byte>)
+    ensures |bs| == 4096*Inode.MAX_SZ
+  {
+    C.concat_homogeneous_len(d.blks, 4096);
+    C.concat(d.blks)
+  }
+
+  function inode_data(sz: nat, d: InodeData): (bs:seq<byte>)
+    requires sz <= Inode.MAX_SZ
+    ensures |bs| == sz as nat
+  {
+    raw_inode_data(d)[..sz]
+  }
+
+  class ByteFilesys
+  {
+    const fs: IndFilesys;
+
+    function Repr(): set<object>
+    {
+      fs.Repr()
+    }
+
+    predicate Valid()
+      reads this.Repr()
+    {
+      && fs.ValidQ()
+    }
+
+    function data(): map<Ino, seq<byte>>
+      reads Repr()
+      requires fs.Valid()
+    {
+      map ino:Ino | ino_ok(ino) :: inode_data(fs.metadata[ino], block_data(fs.data)[ino])
+    }
+
+    function raw_data(ino: Ino): seq<byte>
+      reads Repr()
+      requires ino_ok(ino)
+      requires fs.Valid()
+    {
+      raw_inode_data(block_data(fs.data)[ino])
+    }
+
+    constructor Init(d: Disk)
+      ensures Valid()
+      ensures data() == map ino: Ino | ino_ok(ino) :: []
+    {
+      var the_fs := BlockFs.New(d);
+      this.fs := the_fs;
+      new;
+    }
+
+    method {:timeLimitMultiplier 2} alignedRead(txn: Txn, ino: Ino, i: Inode.Inode, off: uint64)
+      returns (bs: Bytes)
+      requires fs.ValidIno(ino, i)
+      requires fs.has_jrnl(txn)
+      requires off % 4096 == 0
+      requires off as nat + 4096 <= 4096*Inode.MAX_SZ
+      ensures bs.data == this.raw_data(ino)[off as nat..off as nat + 4096]
+      ensures fresh(bs)
+    {
+      var blkoff: nat := (off/4096) as nat;
+      bs := BlockFs.Read(this.fs, txn, ino, i, blkoff);
+      ghost var d := block_data(fs.data)[ino];
+      assert bs.data == d.blks[blkoff];
+      C.concat_homogeneous_one_list(d.blks, blkoff, 4096);
+      assert off as nat == 4096*blkoff;
+      assert off as nat + 4096 == 4096*blkoff + 4096;
+      // TODO: this is super slow even though it matches the postcondition of
+      // C.concat_homogeneous_one_list, up to congruence
+      assert d.blks[blkoff] == C.concat(d.blks)[off as nat..off as nat + 4096];
+      // TODO: this is slow even with the above assumed
+      assert bs.data == this.raw_data(ino)[off as nat..off as nat + 4096] by {
+        reveal raw_inode_data();
+      }
+    }
+
+    method readInternal(txn: Txn, ino: Ino, i: Inode.Inode, off: uint64, len: uint64)
+      returns (bs: Bytes)
+      requires fs.ValidIno(ino, i)
+      requires fs.has_jrnl(txn)
+      requires 0 < len
+      requires off as nat + len as nat <= |data()[ino]|
+      ensures fresh(bs)
+      ensures bs.data == this.data()[ino][off..off+len]
+    {
+      var off' := off / 4096 * 4096;
+      assert off' + 4096 <= 4096*Inode.MAX_SZ_u64 by {
+        Arith.div_incr(off' as nat, Inode.MAX_SZ, 4096);
+      }
+      bs := alignedRead(txn, ino, i, off');
+      assume false;
+      if off' + 4096 >= off + len {
+        // we finished the entire read
+        bs.Subslice(off % 4096, off % 4096 + len);
+        fs.finishInodeReadonly(ino, i);
+        var _ := txn.Commit();
+        C.double_subslice_auto(data()[ino]);
+        return;
+      }
+    }
+
+    // TODO: why is this so slow?
+    method {:timeLimitMultiplier 2} Read(ino: Ino, off: uint64, len: uint64)
+      returns (bs: Bytes, ok: bool)
+      modifies fs.fs
+      requires Valid() ensures Valid()
+      requires ino_ok(ino)
+      ensures ok ==>
+          && off as nat + len as nat <= |data()[ino]|
+          && bs.data == this.data()[ino][off..off+len]
+    {
+      if len > 4096 {
+        ok := false;
+        bs := NewBytes(0);
+        return;
+      }
+      var txn := fs.fs.jrnl.Begin();
+      var i := fs.startInode(txn, ino);
+
+      if sum_overflows(off, len) || off+len > i.sz {
+        ok := false;
+        bs := NewBytes(0);
+        fs.finishInodeReadonly(ino, i);
+        return;
+      }
+      assert off as nat + len as nat <= |data()[ino]|;
+
+      ok := true;
+      if len == 0 {
+        bs := NewBytes(0);
+        fs.finishInodeReadonly(ino, i);
+        calc {
+          this.data()[ino][off..off+len];
+          { assert off+len == off; }
+          this.data()[ino][off..off];
+          [];
+          bs.data;
+        }
+        return;
+      }
+      assert 0 < len <= 4096;
+      bs := readInternal(txn, ino, i, off, len);
+      fs.finishInodeReadonly(ino, i);
+      assert data() == old(data());
+      var _ := txn.Commit();
+    }
+
+  }
+}
